Experimenting with typed state handling

examples/effect_handling/IntSTHandler.fst
@@ -4,9 +4,20 @@ open IntST
 
 open FStar.Heap
 open FStar.ST
-open FStar.Tactics
 
+open FStar.List
 open FStar.Printf
+
+assume type a
+assume val test_return_value : a
+
+let prog_type = unit
+
+let prog : st prog_type = 
+  //IntST.return test_return_value
+  //IntST.get ()
+  //s <-- IntST.get ();
+  IntST.put 42
 
 (* *********************************************** *)
 
@@ -24,6 +35,8 @@ let handle_put (r:ref int) (i:int) : ST unit (requires (fun _ -> True))
 
 (* *********************************************** *)
 
+open FStar.Tactics
+
 let rec collect_app_ref' (ref:term) (args:list (a:argv{a << ref})) (t:term{t == ref \/ t << ref}) 
   : Tot (t:term{t == ref \/ t << ref} * list (a:argv{a << ref})) (decreases t) =
   match inspect t with
@@ -40,56 +53,136 @@ let rec args_wo_ref #ref args =
   | [] -> []
   | a::args -> a :: args_wo_ref args
 
-val handle_st : #a:Type -> st a -> ref int -> tactic term
-let handle_st #a f r = 
+let rec handle_st_typed (a:Type) (f:st a) (r:ref int) : tactic (unit -> ST a (requires (fun _ -> True)) 
+                                                                             (ensures  (fun h0 x h1 -> (x,sel h1 r) == f (sel h0 r)))) =
   t <-- quote f;
-  r <-- quote r;
-  t <-- norm_term [delta_only ["IntSTHandler.prog"]] t;
 
-  t_ret <-- quote IntST.return;
-  t_get <-- quote IntST.get;
-  t_put <-- quote IntST.put;
+  t_return  <-- quote IntST.return;
+  t_bind    <-- quote IntST.bind;
+  t_get     <-- quote IntST.get;
+  t_put     <-- quote IntST.put;
+
+  match inspect t with
+  | Tv_App _ _ ->
+      let (t_fun,args) = collect_app_ref t t in
+
+      if (term_eq t_fun t_return && length args = 2) 
+        then (t_fun <-- quote handle_return;
+              t_ref <-- quote r;
+              let args = [t_ref,Q_Explicit;
+                          FStar.List.Tot.Base.index args 0;
+                          FStar.List.Tot.Base.index args 1] in              
+              ty <-- quote Prims.unit;
+              let t_out = pack (Tv_Abs (fresh_binder ty) (mk_app t_fun args)) in
+              unquote t_out)
+
+      else if (term_eq t_fun t_bind && length args = 4) 
+        then (//a1 <-- unquote #Type (fst (FStar.List.Tot.Base.index args 0));
+              //f1 <-- unquote #a1 (fst (FStar.List.Tot.Base.index args 2));
+              //t1 <-- handle_st_typed a1 f1 r;
+              fail "bind case not yet implemented")
+
+      else if (term_eq t_fun t_get && length args = 1) 
+        then (t_fun <-- quote handle_get;
+              t_ref <-- quote r;
+              let args = [t_ref,Q_Explicit] in              
+              ty <-- quote Prims.unit;
+              let t_out = pack (Tv_Abs (fresh_binder ty) (mk_app t_fun args)) in
+              unquote t_out)
+
+      else if (term_eq t_fun t_put && length args = 1) 
+        then (t_fun <-- quote handle_put;
+              t_ref <-- quote r;
+              let args = [t_ref,Q_Explicit;
+                          FStar.List.Tot.Base.index args 0] in              
+              ty <-- quote Prims.unit;
+              let t_out = pack (Tv_Abs (fresh_binder ty) (mk_app t_fun args)) in
+              unquote t_out)
+
+      else fail "application case not implemented"
+
+  | _ -> fail "case not implemented"
+
+let synth_prog_typed (r:ref int) : unit -> ST prog_type (requires (fun _ -> True)) 
+                                                        (ensures  (fun h0 x h1 -> (x,sel h1 r) == prog (sel h0 r))) 
+  = synth_by_tactic
+    (
+      t <-- quote prog;      
+      t <-- norm_term [delta_only ["IntSTHandler.prog"]] t;
+      t <-- unquote #(st prog_type) t;
+      t <-- handle_st_typed prog_type t r;
+      t <-- quote t;
+      print (term_to_string t);;
+      exact (return t)
+    )
+
+
+
+(* ********************************************************** *)
+
+
+(* untyped handling experiment *)
+
+(*let rec handle_st (t:term) (r:term) : tactic term = 
+  t_return  <-- quote IntST.return;
+  t_bind    <-- quote IntST.bind;
+  t_get     <-- quote IntST.get;
+  t_put     <-- quote IntST.put;
 
   match inspect t with
   | Tv_App _ _ ->
       let (t_fun,args) = collect_app_ref t t in
 
       // Handle IntST.return with handle_return (i.e., with ST's return)
-      if (term_eq t_fun t_ret) then (t_fun <-- quote handle_return;
-                                     let args = (r,Q_Explicit)::(args_wo_ref args) in
-                                     return (mk_app t_fun args))
+      if (term_eq t_fun t_return && length args = 2) 
+        then (t_fun <-- quote handle_return;
+              let args = [r,Q_Explicit;
+                          FStar.List.Tot.Base.index args 0;
+                          FStar.List.Tot.Base.index args 1] in
+              return (mk_app t_fun args))
+
+      // Handle IntST.bind
+      else if (term_eq t_fun t_bind && length args = 4) 
+        then (let t0 = fst (FStar.List.Tot.Base.index args 2) in
+              t0 <-- handle_st t0 r;
+              let t1 = fst (FStar.List.Tot.Base.index args 3) in
+              match inspect t1 with 
+              | Tv_Abs b t1 -> t1 <-- handle_st t1 r;
+                               return (pack (Tv_Let b t0 t1))
+              | _ -> fail "body of bind is not a lambda")
 
       // Handle IntST.get_st with handle_get (i.e., with ST's read)
-      else if (term_eq t_fun t_get) then (t_fun <-- quote handle_get; 
-                                          let args = [r,Q_Explicit] in
-                                          return (mk_app t_fun args))
+      else if (term_eq t_fun t_get && length args = 1) 
+        then (t_fun <-- quote handle_get; 
+              let args = [r,Q_Explicit] in
+              return (mk_app t_fun args))
 
       // Handle IntST.put_st with handle_put (i.e., with ST's write)
-      else if (term_eq t_fun t_put) then (t_fun <-- quote handle_put; 
-                                          let args = (r,Q_Explicit)::(args_wo_ref args) in
-                                          return (mk_app t_fun args))
+      else if (term_eq t_fun t_put && length args = 1) 
+        then (t_fun <-- quote handle_put; 
+              let args = [r,Q_Explicit;
+                          FStar.List.Tot.Base.index args 0] in
+              return (mk_app t_fun args))
 
       else fail "not implemented application case"
   | _ -> fail "not implemented case"
-
-let prog_type = int
-
-let prog : st prog_type = 
-  //IntST.return 0
-  IntST.get ()
-  //IntST.put 42
 
 let synth_prog (r:ref int) : unit -> ST prog_type (requires (fun _ -> True)) 
                                                   (ensures  (fun h0 x h1 -> (x,sel h1 r) == prog (sel h0 r))) 
   = synth_by_tactic
     (
-      t  <-- handle_st prog r;
+      t <-- quote prog;      
+      r <-- quote r;
+
+      t <-- norm_term [delta_only ["IntSTHandler.prog"]] t;
+
+      t  <-- handle_st t r;
       ty <-- quote Prims.unit;
       let f = pack (Tv_Abs (fresh_binder ty) t) in
-      //print (term_to_string f);;
+
       exact (return f)
     )
-
+*)
 
 
 
